lander1

CaseStudies/lander/Lander1.thy
@@ -1,22 +1,12 @@
 
 theory Lander1
-    imports HHLProver.HHLProver
+  imports HHLProver.HHLProver
 begin
 
-definition landerinv :: "real \<Rightarrow> real \<Rightarrow> real \<Rightarrow> real \<Rightarrow> real" where
-"landerinv t V F m = (-1139598426176000000000*F^2 + 6016579819909859424000*F*m - 
- 15025282795421706426953*m^2 + 6579819920896000000000*F^2*t - 
- 32152462695621728000000*F*m*t + 38191371615549881350000*m^2*t - 
- 63926169690400000000*F*m*t^2 - 9482947285373987200000*m^2*t^2 + 
- 90382078252408000000*m^2*t^3 + 12597135205472000000*m^2*t^4 - 
- 1659591880613072768000*F*m*V - 5070724623344300111384*m^2*V + 
- 11298598523808000000000*F*m*t*V - 29051341984741759604000*m^2*t*V - 
- 12905500940447680000000*m^2*t^2*V + 3452247087952000000*m^2*t^3*V - 
- 2216823024256000*F*m*V^2 - 3754952256975690758168*m^2*V^2 + 
- 4369639740028640264000*m^2*t*V^2 - 
- 4290324517728000000000*m^2*t^2*V^2 - 10509874347360*m^2*V^3 + 
- 8711967253392000*m^2*t*V^3 - 1751645724560*m^2*V^4)/(1/(160000000000000000000*m^2))"
 
+lemma frontier_closed_open:
+  "frontier {s. f s \<ge> a \<and> f s < b} = {s. f s = b}"
+  sorry
 
 text \<open>Variables\<close>
 
@@ -24,33 +14,132 @@ definition Fc :: char where "Fc = CHR ''a''"
 definition M :: char where "M = CHR ''b''"
 definition T :: char where "T = CHR ''c''"
 definition V :: char where "V = CHR ''d''"
+definition W :: char where "W = CHR ''e''"
 
+text \<open>Constants\<close>
+definition Period :: real where "Period = 0.128"
+
+lemma train_vars_distinct [simp]: "T \<noteq> V" "T \<noteq> W"  
+                                  "V \<noteq> T" "V \<noteq> W" 
+                                  "W \<noteq> T" "W \<noteq> V" 
+  unfolding T_def V_def W_def by auto
+
+
+definition W_upd :: "real \<Rightarrow> real \<Rightarrow> real" where
+  "W_upd v w = (-(w - 3.732) * 0.01 + 3.732 - (v - (-1.5)) * 0.6)"
+
+definition landerinv :: "real \<Rightarrow> real \<Rightarrow> real \<Rightarrow> real" where
+"landerinv t v w = (15025282795421706426953 - 38191371615549881350000*t + 
+  9482947285373987200000*t^2 - 90382078252408000000*t^3 - 
+  12597135205472000000*t^4 + 5070724623344300111384 * v + 
+  29051341984741759604000 * t * v + 12905500940447680000000*t^2 * v - 
+  3452247087952000000*t^3 * v + 3754952256975690758168 * v^2 - 
+  4369639740028640264000*t * v^2 + 4290324517728000000000*t^2 * v^2 + 
+  10509874347360 * v^3 - 8711967253392000*t * v^3 + 1751645724560 * v^4 - 
+  6016579819909859424000*w + 32152462695621728000000*t*w + 
+  63926169690400000000*t^2*w + 1659591880613072768000 * v *w - 
+  11298598523808000000000*t * v *w + 2216823024256000 * v^2*w + 
+  1139598426176000000000*w^2 - 6579819920896000000000*t*w^2)/(160000000000000000000)"
+
+
+lemma landerinv_prop2:
+  "landerinv Period v w \<le> 0 \<Longrightarrow> landerinv 0 v (W_upd v w) \<le> 0"
+  sorry
+
+definition landerInv :: "state \<Rightarrow> real" where
+  "landerInv s = landerinv (s T) (s V) (s W)"
 
 text \<open>Processes\<close>
 
+(*
+  V ::= (\<lambda>_. -1.5);
+  W ::= (\<lambda>_. 2835/759.5);
+*)
 definition P0 :: proc where
   "P0 =
-    Fc ::= (\<lambda>_. 2835);
-    V ::= (\<lambda>_. -1.5);
-    M ::= (\<lambda>_. 759.5);
     Rep (
-      Fc ::= (\<lambda>s. (-(s Fc / s M - 3.732) * 0.01 + 3.732 - (s V - (-1.5)) * 0.6) * s M);
       T ::= (\<lambda>_. 0);
-      Cont (ODE ((\<lambda>_ _. 0)(V := (\<lambda>s. s Fc / s M - 3.732), M := (\<lambda>s. s Fc / 2500 * (-1)), T := (\<lambda>_. 1)))) ((\<lambda>s. s T < 0.128))
+      Cont (ODE ((\<lambda>_ _. 0)(V := (\<lambda>s. s W - 3.732),
+                           W := (\<lambda>s. (s W)^2 / 2500 ),
+                           T := (\<lambda>_. 1)))) ((\<lambda>s. s T \<ge> 0 \<and> s T < Period));
+      W ::= (\<lambda>s. W_upd (s V) (s W))
     )"
 
-lemma test:
-  fixes a :: real and 
-    b :: real
-  shows "a\<^sup>2 + 2 * a * b + b\<^sup>2 \<ge> 0"
-  by sos
+fun P0_inv :: "nat \<Rightarrow> tassn" where
+  "P0_inv 0 = emp\<^sub>t"
+| "P0_inv (Suc n) = (ode_inv_assn (\<lambda>s. landerInv s \<le> 0) @\<^sub>t P0_inv n)"
 
-lemma test2:
-  fixes a :: real and 
-    b :: real
-  shows "0.386144 * a\<^sup>2 + 0.342381 * a * b + 0.174365 * b\<^sup>2 \<ge> 0"
-  by sos
+lemma P0_inv_Suc:
+  "P0_inv n @\<^sub>t ode_inv_assn (\<lambda>s. landerInv s \<le> 0) = 
+   ode_inv_assn (\<lambda>s. landerInv s \<le> 0) @\<^sub>t P0_inv n"
+  apply (induct n) by (auto simp add: join_assoc)
+
+lemma ContODE:
+ "\<Turnstile> {\<lambda>s tr. landerInv s \<le> 0 \<and>
+             (\<lambda>s. s T \<ge> 0 \<and> s T < Period) s \<and>
+             supp s \<subseteq> {V, W, T} \<and> P tr}
+     Cont (ODE ((\<lambda>_ _. 0)(V := (\<lambda>s. s W - 3.732), W := (\<lambda>s. (s W)^2 / 2500 ), T := (\<lambda>_. 1)))) ((\<lambda>s. s T \<ge> 0 \<and> s T < Period))
+    {\<lambda>s tr. s \<in> frontier {s. s T \<ge> 0 \<and> s T < Period} \<and>
+            supp s \<subseteq> {V, W, T} \<and>
+            landerInv s \<le> 0 \<and>
+            (P @\<^sub>t ode_inv_assn (\<lambda>s. landerInv s \<le> 0)) tr}"
+  apply(rule Valid_inv_new')
+   apply auto
+  unfolding landerInv_def landerinv_def vec2state_def power2_eq_square power3_eq_cube power4_eq_xxxx
+   apply(rule has_derivative_divide)
+     apply (fast intro!: derivative_intros)[1]
+    apply (fast intro!: derivative_intros)[1]
+  apply auto
+  apply(simp add:state2vec_def Period_def)
+  subgoal for S
+    sorry
+  done
 
 
-
+lemma P0_prop:
+  "\<Turnstile> {\<lambda>s tr. s = (\<lambda>_. 0)(V := v0, W := w0, T := Period) \<and>
+                  landerinv 0 v0 w0 \<le> 0 \<and> emp\<^sub>t tr}
+     P0
+   {\<lambda>s tr. \<exists>n v w. s = (\<lambda>_. 0)(V := v, W := w, T := Period) \<and>
+                   landerinv 0 v w \<le> 0 \<and> P0_inv n tr}"
+  unfolding P0_def
+  apply (rule Valid_weaken_pre)
+   prefer 2
+  apply (rule Valid_rep)
+  apply (rule Valid_ex_pre) apply (rule Valid_ex_pre)
+  apply (rule Valid_ex_pre)
+  subgoal for n v w
+    apply (rule Valid_seq)
+     apply (rule Valid_assign_sp)
+    apply (rule Valid_seq)
+     apply (rule Valid_weaken_pre)
+      prefer 2 
+    apply (rule ContODE[where P="P0_inv n"])
+     apply auto
+     apply (auto simp add: entails_def landerInv_def supp_def Period_def)[1]
+    apply (rule Valid_weaken_pre[where P'=
+          "\<lambda>s tr. \<exists>v w. s = ((\<lambda>_. 0)(V := v, W := w, T := Period)) \<and>
+                        landerInv s \<le> 0 \<and>
+                        (P0_inv n @\<^sub>t ode_inv_assn (\<lambda>s. landerInv s \<le> 0)) tr"])
+    subgoal
+      apply (auto simp add: entails_def frontier_closed_open supp_def)
+      subgoal for s tr
+        apply (rule exI[where x="s V"]) apply (rule exI[where x="s W"])
+        apply (rule ext) by auto
+      done
+    apply (rule Valid_ex_pre)
+    apply (rule Valid_ex_pre)
+    subgoal for v w
+    apply (rule Valid_strengthen_post)
+       prefer 2 apply (rule Valid_assign_sp)
+      apply (auto simp add: entails_def)
+      apply (rule exI[where x="Suc n"])
+      apply (rule exI[where x=v]) apply (rule exI[where x="W_upd v w"])
+      apply (auto simp add: P0_inv_Suc)
+      by (auto simp add: landerInv_def landerinv_prop2)
+    done
+  apply (auto simp add: entails_def)
+  apply (rule exI[where x=0]) apply (rule exI[where x=v0])
+  apply (rule exI[where x=w0]) by auto
+  
 end
