lunarlander_sl/ContinuousInv.thy
@@ -13,9 +13,27 @@ proof -
   have 2: "0 \<le> t \<and> t \<le> d"
     using assms(3) by auto
   have 3: "((\<lambda>t. state2vec(p t)) has_derivative (\<lambda>s. s *\<^sub>R ODE2Vec ode (p t))) (at t within {0..d})"
-    using 2 assms(2) unfolding ODEsol_def has_vderiv_on_def has_vector_derivative_def by auto
+    using 2 assms(2) using ODEsol_old[OF assms(2)]unfolding ODEsol_def has_vderiv_on_def has_vector_derivative_def by auto
   show ?thesis
   using 1 2 3 has_derivative_in_compose2[of UNIV "(\<lambda>v. g (vec2state v))" "(\<lambda>v. g' (vec2state v))" "(\<lambda>t. state2vec (p t))" "{0 .. d}" t "(\<lambda>s. s *\<^sub>R ODE2Vec ode (p t))"]
+  by auto
+qed
+
+lemma chainrule':
+  assumes "\<forall>x. ((\<lambda>v. g (vec2state v)) has_derivative g' (vec2state x)) (at x within UNIV)"
+    and "((\<lambda>t. state2vec (p t)) has_vderiv_on (\<lambda>t. ODE2Vec ode (p t))) {-e .. d+e}"
+    and "e>0"
+    and "t \<in> {-e .. d+e}"
+  shows "((\<lambda>t. g (p t)) has_derivative (\<lambda>s. g' (p t) (s *\<^sub>R ODE2Vec ode (p t)))) (at t within {-e .. d+e})"
+proof -
+  have 1: "(\<And>x. x \<in> UNIV \<Longrightarrow> ((\<lambda>v. g (vec2state v)) has_derivative g' (vec2state x)) (at x))"
+    using assms(1) by auto
+  have 2: "-e \<le> t \<and> t \<le> d+e"
+    using assms(3) assms(4) by auto
+  have 3: "((\<lambda>t. state2vec(p t)) has_derivative (\<lambda>s. s *\<^sub>R ODE2Vec ode (p t))) (at t within {-e .. d+e})"
+    using 2 assms(2) unfolding ODEsol_def has_vderiv_on_def has_vector_derivative_def by auto
+  show ?thesis
+  using 1 2 3 has_derivative_in_compose2[of UNIV "(\<lambda>v. g (vec2state v))" "(\<lambda>v. g' (vec2state v))" "(\<lambda>t. state2vec (p t))" "{-e .. d+e}" t "(\<lambda>s. s *\<^sub>R ODE2Vec ode (p t))"]
   by auto
 qed
 
@@ -95,5 +113,97 @@ theorem Valid_inv':
     done
   done
 
+definition supp :: "state \<Rightarrow> var set" where
+  "supp s = {v. s v \<noteq> 0}"
+
+fun ode_supp :: "ODE \<Rightarrow> var set" where
+  "ode_supp (ODE ode) = {v. ode v \<noteq> (\<lambda>_. 0)}"
+
+theorem Valid_inv_new':
+  fixes inv :: "state \<Rightarrow> real"
+  assumes "\<forall>x. ((\<lambda>v. inv (vec2state v)) has_derivative g' (x)) (at x within UNIV)"
+    and "\<forall>S. b S \<longrightarrow> ((inv S = 0) \<longrightarrow> g' (state2vec S) (ODE2Vec (ODE ode) S) < 0)"
+    and "ode_supp (ODE ode) \<subseteq> VS" 
+  shows "\<Turnstile> {\<lambda>s tr. inv s \<le> 0 \<and> b s \<and> supp s \<subseteq> VS \<and> P tr}
+     Cont (ODE ode) b
+    {\<lambda>s tr. s \<in> frontier {s. b s} \<and> supp s \<subseteq> VS \<and> inv s \<le> 0 \<and>
+            (P @\<^sub>t ode_inv_assn (\<lambda>s. inv s \<le> 0)) tr}"
+  unfolding Valid_def
+  apply (auto elim!: contE)
+  subgoal for tr1 d p
+    sorry
+  subgoal for tr1 d p v
+    unfolding supp_def apply auto
+    subgoal premises pre
+    proof(rule ccontr)
+      assume cond:"v \<notin> VS"
+     have 1:"p 0 v = 0" using pre cond by auto
+     have 2:"ode v = (\<lambda>_. 0)"
+       using assms(3) cond by auto
+     have 3:"((\<lambda>t. p t v) has_vderiv_on (\<lambda>t. 0)) {0 .. d}"
+       using ODEsol_old[OF pre(5)]
+       using has_vderiv_on_proj[of "(\<lambda>t. state2vec (p t))" "(\<lambda>t. ODE2Vec (ODE ode) (p t))"  "{0 .. d}" v]
+       apply auto
+       unfolding state2vec_def apply auto
+       using 2 by auto
+     then have 4:"p 0 v = p d v"
+       unfolding has_vderiv_on_def has_vector_derivative_def
+       using mvt_real_eq[of d "(\<lambda>t. p t v)" "\<lambda>t. (\<lambda>x. x *\<^sub>R 0)" d] 
+       using pre by auto
+     then show False using 1 pre by auto
+   qed
+   done
+  subgoal premises pre for tr1 d p
+    proof-
+     obtain e where e: "e > 0" "((\<lambda>t. state2vec (p t)) has_vderiv_on (\<lambda>t. ODE2Vec (ODE ode) (p t))) {-e .. d+e}"
+       using pre unfolding ODEsol_def by auto
+    have 1: "\<forall>t\<in>{-e .. d+e}. ((\<lambda>t. inv(p t)) has_derivative  (\<lambda>s. g' (state2vec(p t)) (s *\<^sub>R ODE2Vec (ODE ode) (p t)))) (at t within {-e .. d+e})"
+        using pre assms e
+        using chainrule'[of inv "\<lambda>x. g'(state2vec x)" p "(ODE ode)" e d] 
+        by auto
+    have 2: "\<forall>s. g' (state2vec(p t)) ((s *\<^sub>R 1) *\<^sub>R ODE2Vec (ODE ode) (p t)) = s *\<^sub>R g' (state2vec(p t)) (1 *\<^sub>R ODE2Vec (ODE ode) (p t))" if "t\<in>{-e .. d+e}" for t
+        using 1 unfolding has_derivative_def bounded_linear_def 
+        using that linear_iff[of "(\<lambda>s. g' (state2vec(p t)) (s *\<^sub>R ODE2Vec (ODE ode) (p t)))"]
+        by blast
+    have 3: "(s *\<^sub>R 1) = s" and "(1 *\<^sub>R s) = s" 
+      apply simp by simp
+      have 4: "\<forall>s. g' (state2vec(p t)) (s *\<^sub>R ODE2Vec (ODE ode) (p t)) = s *\<^sub>R g' (state2vec(p t)) (ODE2Vec (ODE ode) (p t))" if "t\<in>{-e .. d+e}" for t
+        using 2 3 that by auto
+      have 5: "inv(p t) = 0 \<longrightarrow>  g' (state2vec(p t)) (ODE2Vec (ODE ode) (p t))< 0" if "t\<in>{0 ..<d}" for t
+        using 4 assms(2) that pre by auto
+      show ?thesis
+        using real_inv_le[OF 1] 
+        using pre 5 e 3 by auto
+    qed
+  subgoal for tr1 d p
+    apply(simp add: join_assn_def)
+    apply(rule exI [where x="tr1"])
+    apply auto
+   apply (auto intro!: ode_inv_assn.intros)
+   subgoal premises pre for \<tau>
+   proof-
+     obtain e where e: "e > 0" "((\<lambda>t. state2vec (p t)) has_vderiv_on (\<lambda>t. ODE2Vec (ODE ode) (p t))) {-e .. d+e}"
+       using pre unfolding ODEsol_def by auto
+    have 1: "\<forall>t\<in>{-e .. d+e}. ((\<lambda>t. inv(p t)) has_derivative  (\<lambda>s. g' (state2vec(p t)) (s *\<^sub>R ODE2Vec (ODE ode) (p t)))) (at t within {-e .. d+e})"
+        using pre assms e
+        using chainrule'[of inv "\<lambda>x. g'(state2vec x)" p "(ODE ode)" e d] 
+        by auto
+    have 2: "\<forall>s. g' (state2vec(p t)) ((s *\<^sub>R 1) *\<^sub>R ODE2Vec (ODE ode) (p t)) = s *\<^sub>R g' (state2vec(p t)) (1 *\<^sub>R ODE2Vec (ODE ode) (p t))" if "t\<in>{-e .. d+e}" for t
+        using 1 unfolding has_derivative_def bounded_linear_def 
+        using that linear_iff[of "(\<lambda>s. g' (state2vec(p t)) (s *\<^sub>R ODE2Vec (ODE ode) (p t)))"]
+        by blast
+    have 3: "(s *\<^sub>R 1) = s" and "(1 *\<^sub>R s) = s" 
+      apply simp by simp
+      have 4: "\<forall>s. g' (state2vec(p t)) (s *\<^sub>R ODE2Vec (ODE ode) (p t)) = s *\<^sub>R g' (state2vec(p t)) (ODE2Vec (ODE ode) (p t))" if "t\<in>{-e .. d+e}" for t
+        using 2 3 that by auto
+      have 5: "inv(p t) = 0 \<longrightarrow>  g' (state2vec(p t)) (ODE2Vec (ODE ode) (p t))< 0" if "t\<in>{0 ..<d}" for t
+        using 4 assms(2) that pre by auto
+      show ?thesis
+        using real_inv_le[OF 1] 
+        using pre 5 e 3 by auto
+    qed
+    done
+  done
+        
 
 end
