lunarlander_sl/ExampleContinuous.thy
@@ -70,6 +70,8 @@ proof -
   have 1: "ODEsol (ODE ((\<lambda>_ _. 0)(X := \<lambda>_. 1))) (\<lambda>t. (\<lambda>_. 0)(X := t + a)) (1 - a)"
      unfolding ODEsol_def solves_ode_def has_vderiv_on_def
      using assms apply auto
+apply(rule exI[where x="1"])
+  apply auto
      apply (rule has_vector_derivative_projI)
      apply (auto simp add: state2vec_def)
      apply (rule has_vector_derivative_eq_rhs)
@@ -108,6 +110,8 @@ proof -
   have 1: "ODEsol (ODE ((\<lambda>_ _. 0)(X := \<lambda>_. 1))) (\<lambda>t. (\<lambda>_. 0)(X := t + a)) (1 - a)"
      unfolding ODEsol_def solves_ode_def has_vderiv_on_def
      using assms apply auto
+apply(rule exI[where x="1"])
+  apply auto
      apply (rule has_vector_derivative_projI)
      apply (auto simp add: state2vec_def)
      apply (rule has_vector_derivative_eq_rhs)
@@ -338,6 +342,8 @@ proof -
   have 1: "ODEsolInf (ODE ((\<lambda>_ _. 0)(X := \<lambda>_. 1))) (\<lambda>t. (\<lambda>_. 0)(X := t + a))"
      unfolding ODEsolInf_def solves_ode_def has_vderiv_on_def
      apply auto
+apply(rule exI[where x="1"])
+  apply auto
      apply (rule has_vector_derivative_projI)
      apply (auto simp add: state2vec_def)
      apply (rule has_vector_derivative_eq_rhs)
